---
layout: default
title: September 3
parent: 658-Lectures
mathjax: true
tags: 
  - latex
  - math
has_children: true
---

# September 3

## Recap
- Problem set 1 is out.
- Should start doing it.
- Due in about 2 weeks from August 28... which is September 11.
- Recall Feynman Lectures

Recall that mean square of something is always greater than square of the mean.

$$
v = \bar v
$$

Or...

$$
\begin{align}
\int_0^T \frac{1}{2} m v^2 dt &\geq \int_0^T \frac{1}{2} m \bar v^2 \space dt \\
\bar v &= \frac{1}{T} \int_0^T v \space dt
\end{align}
$$

I can prove this haha...

$$
\begin{align*}
\text{LHS} &= \frac{1}{2} m \int_0^T v^2 dt \\
\text{RHS} &= \int_0^T \frac{1}{2} m (\frac{1}{T} \int_0^T v \space dt)^2 \space dt \\
&= \int_0^T \frac{1}{2} m \frac{1}{T^2} (\int_0^T v \space dt)^2 \space dt \\
&= \frac{1}{2} m \int_0^T \frac{1}{T^2} (\int_0^T v \space dt)^2 \space dt \\
&= \frac{1}{2} m \frac{1}{T} (\int_0^T v \space dt)^2\\
\end{align*}
$$

Least Action
$$
\begin{align}
T = \frac{1}{2} \dot q^T G \dot q \\
p = G \dot q \\
\dot q = G^{-1} p
\end{align}
$$

$$
\begin{align*}
\delta \int_q L(q,\dot q) \space dt = 0 \\
q(b) = q_b \\
q(a) = q_a \\
q(t,0) = q(t), \space t \in [a,b] \\
q(t,a) = q_a \\
q(t,b) = q_b \\
\delta q (t) = \frac{\partial}{\partial t} q(t, \epsilon) |_{\epsilon = 0} ... \text{- virtual displacement}
\end{align*}
$$

$$
\begin{align*}
\frac{d}{dt} \int_a^b L(q(t,\epsilon), \dot q(t,\epsilon)) \space dt |_{\epsilon = 0} &= 0 \\
q(t) \text{ is a critical curve}
\end{align*}
$$

**Proposition**: $$\frac{d}{dt} (\frac{\partial L}{\partial q^i}) - \frac{\partial L}{\partial q^i} = 0$$

$$
\begin{align*}
q(t,\epsilon) = q(t,0) + \epsilon \\
\text{see Feynman or Goldstein}
\end{align*}
$$

Feynman thesis moves least action principle to quantum mechanics.

Now we extend to Lagrange d'Alembert Principle...

$$
\begin{align*}
\frac{d}{dt} (\frac{\partial L}{\partial q^i}) - \frac{\partial L}{\partial q^i} = F_i \\
F_i \text{ is generalized force external to system.}
\end{align*}
$$

One example of $$F_i$$ is friction.
Another example is $$ non-holonomic constraint forces.

Nonholonomic example:

$$
\begin{align}
\dot x = R \cos \rho \dot \theta \\
\dot y = R \sin \rho \dot \theta \\ 
\sum_{k=1}^n a^i_k(a), \dot q^k = 0, j=1,...,m \\
\exists b^j(q) \text{s.t.} \\
\sum_{k=1}^n \frac{\partial b^i}{\partial q^k} \dot q^k = 0 \text{ - holonomic}
\end{align}
$$

The force of constraint will keep a non-holonomic system (like a penny rolling on a table) that keeps the penny upright on the table.

$$F_i \delta q^1 + ... + F_m \delta q^m = 0$$.

Forces of constraint do no work.

Now plug into EoM

$$
\begin{align*}
\frac{d}{dt} (\frac{\partial L}{\partial q^i}) - \frac{\partial L}{\partial q^i} = \sum_{j=1}^m \lambda_j a_i^j
\end{align*}
$$

where $$\lambda_j$$ are the Lagrange multipliers associated with the constraints and $$a_i^j$$ are the constraints.

And thus 

$$
\begin{align*}
F_i = a^i_1 + ... + \lambda_m a_i^m \\
F_i \perp ker(A)
\end{align*}
$$

The last statement is just another way of saying that $$F_i$$ should be in the range of constraint matrix. It cannot lie in the nullspace (thus has to be perpendicular).

Now lets look at an example problem:

$$
\begin{align*}
L = \frac{1}{2}m(\dot x^2 + \dot y^2) + \frac{1}{2} I \dot \theta^2 + \frac{1}{2}J \rho ^2 \\
\dot x = R \cos \rho \dot \theta \\
\dot y = R \sin \rho \dot \theta
\end{align*}
$$

Constraints:

$$
\begin{align*}
\delta x = R \cos \rho \delta \theta \\
\delta y = R \sin \rho \delta \theta
\end{align*}
$$

Substitute into the Lagrangian:

$$
\begin{align*}
L = \frac{1}{2}(\dot x^2 + \dot y^2) + \frac{1}{2} I \dot \theta^2 + \frac{1}{2}J \rho ^2 \\
\dot x = R \cos \rho \dot \theta \\
\dot y = R \sin \rho \dot \theta
\end{align*}
$$

Constraints:

$$
\begin{align*}
\delta x = R \cos \rho \delta \theta \\
\delta y = R \sin \rho \delta \theta
\end{align*}
$$

Now our EoM is this when throwing in $$\frac{d}{dt}$$.

$$
\begin{align}
m \ddot x \delta x + m \ddot y \delta y + I \ddot \theta \delta \theta + J \ddot \rho \delta \rho = 0
\end{align}
$$

Now replace $$\delta$$.

$$
\begin{align}
m \ddot x (R \cos \rho \delta \theta) + m \ddot y (R \sin \rho \delta \theta) + I \ddot \theta \delta \theta + J \ddot \rho \delta \rho = 0
\end{align}
$$

Set coeffs of $$\delta \theta$$ and $$\delta \rho$$ to 0.

$$
\begin{align}
J \ddot \rho = 0 \\
m \ddot x (R \cos \rho) + m \ddot y (R \sin \rho) + I \ddot \theta = 0
\end{align}
$$

**TAKEAWAY**: can think of external forces as ones that come from constraints....


## ODE's

**Def'n**: A dynamical system is a $$C^1$$ map $$\mathbb{R} \times S \mapsto \phi$$ where $$S$$ is an open set of euclidian space (eventually we'll do manifold).  $$\phi(t,x) = \phi_t(x)$$.

s.t.

- flow $$\phi_0: S \mapsto S$$
- flow composition $$ \phi_t \circ \phi_s = \phi_{t+s}$$

For a linear system, $$e^{At}$$ is the flow of $$\dot x = Ax$$.

Fundamental theorem of ODE's.